Utilities/BasicComputation.thy
@@ -3,11 +3,21 @@ imports Main
 begin
 
 typedecl code_label
+typedecl function_name
 
 axiomatization new_label :: "code_label set \<Rightarrow> code_label" where
   new_fresh [simp]: "finite ss \<Longrightarrow> new_label ss \<notin> ss"
 
+datatype code_label\<^sub>2 = CL\<^sub>2 function_name code_label
+
+axiomatization new_label\<^sub>2 :: "code_label\<^sub>2 set \<Rightarrow> code_label\<^sub>2" where
+  new_fresh\<^sub>2 [simp]: "finite ss \<Longrightarrow> new_label\<^sub>2 ss \<notin> ss"
+
 type_synonym "output" = "int list"
+
+primrec repeat :: "'a \<Rightarrow> nat \<Rightarrow> 'a list" where
+  "repeat a 0 = []"
+| "repeat a (Suc n) = a # repeat a n"
 
 definition boolify :: "int \<Rightarrow> bool" where
   "boolify i = (i \<noteq> 0)"
