BranchingAssembly/BranchingAssemblyLanguage.thy
@@ -6,11 +6,12 @@ datatype b_assembly =
   ABAssm int
 | CBAssm "register set" computation
 | IBAssm "comparison set" "b_assembly list" "b_assembly list"
+| JBAssm code_label\<^sub>2
 | PBAssm
 
-type_synonym b_assembly_program = "code_label \<rightharpoonup> b_assembly list \<times> code_label"
+type_synonym b_assembly_program = "code_label\<^sub>2 \<rightharpoonup> b_assembly list \<times> code_label\<^sub>2"
 
-type_synonym b_assembly_state = "memory \<times> int option \<times> int \<times> b_assembly list \<times> code_label \<times> output" 
+type_synonym b_assembly_state = "memory \<times> int option \<times> int \<times> b_assembly list \<times> code_label\<^sub>2 \<times> output" 
   (* \<mu>, a, d, \<pi>, s, \<omega> *)
 
 fun eval_b_assembly :: "b_assembly_program \<Rightarrow> b_assembly_state \<Rightarrow> b_assembly_state option" where
@@ -29,6 +30,10 @@ fun eval_b_assembly :: "b_assembly_program \<Rightarrow> b_assembly_state \<Righ
 | "eval_b_assembly \<Pi> (\<mu>, None, d, CBAssm dst cmp # \<pi>, s, \<omega>) = None"
 | "eval_b_assembly \<Pi> (\<mu>, a, d, IBAssm jmp \<pi>\<^sub>t \<pi>\<^sub>f # \<pi>, s, \<omega>) = 
     Some (\<mu>, None, d, (if compare d jmp then \<pi>\<^sub>t else \<pi>\<^sub>f) @ \<pi>, s, \<omega>)"
+| "eval_b_assembly \<Pi> (\<mu>, a, d, JBAssm s # \<pi>, s', \<omega>) = (
+    case \<Pi> s of 
+      Some (\<pi>', s') \<Rightarrow> Some (\<mu>, None, d, \<pi>', s', \<omega>)
+    | None \<Rightarrow> None)"
 | "eval_b_assembly \<Pi> (\<mu>, a, d, PBAssm # \<pi>, s, \<omega>) = Some (\<mu>, a, d, \<pi>, s, d # \<omega>)"
 
 fun b_assembly_output :: "b_assembly_state \<Rightarrow> output" where
